Continue

src/verification/semantics/skip_stream_multiply.lean
@@ -1,8 +1,29 @@
 import verification.semantics.skip_streamv2
 
-lemma prod.rprod_iff {α β : Type*} {r₁ : α → α → Prop} {r₂ : β → β → Prop} {s₁ s₂ : α × β} :
-  (prod.rprod r₁ r₂ s₁ s₂) ↔ r₁ s₁.1 s₂.1 ∧ r₂ s₁.2 s₂.2 :=
-⟨by { rintro ⟨h⟩, split; assumption, }, by { rintro ⟨h₁, h₂⟩, cases s₁, cases s₂, exact prod.rprod.intro h₁ h₂, }⟩  
+namespace prod
+variables {α β : Type*} (r₁ : α → α → Prop) (r₂ : β → β → Prop)
+
+def rprod_eq (s₁ s₂ : α × β) : Prop :=
+(r₁ s₁.1 s₂.1 ∧ (r₂ s₁.2 s₂.2 ∨ s₁.2 = s₂.2)) ∨
+  (r₂ s₁.2 s₂.2 ∧ (r₁ s₁.1 s₂.1 ∨ s₁.1 = s₂.1))
+
+variables {r₁ r₂}
+
+theorem rprod_eq_sub_lex (s₁ s₂ : α × β) (h : rprod_eq r₁ r₂ s₁ s₂) :
+  prod.lex r₁ r₂ s₁ s₂ :=
+begin
+  cases s₁ with a b, cases s₂ with c d,
+  rcases h with (⟨h₁, _⟩|⟨h₁, (h₂|h₂)⟩),
+  { exact prod.lex.left _ _ h₁, },
+  { exact prod.lex.left _ _ h₂, },
+  { dsimp only at h₁ h₂, rw h₂, exact prod.lex.right _ h₁, }
+end
+
+theorem rprod_eq_wf (h₁ : well_founded r₁) (h₂ : well_founded r₂) :
+  well_founded (rprod_eq r₁ r₂) :=
+subrelation.wf rprod_eq_sub_lex (lex_wf h₁ h₂)
+
+end prod
 
 variables {ι : Type} [linear_order ι] {α : Type*}
 
@@ -14,6 +35,8 @@ structure Stream.mul.ready {ι : Type} (a : Stream ι α) (b : Stream ι α) (s 
 (r₂ : b.ready s.2)
 (index : a.index s.1 v₁ = b.index s.2 v₂)
 
+local notation a ` ≺ `:50 b := Stream.wf_rel _ a b 
+
 @[simps]
 instance [has_mul α] : has_mul (Stream ι α) := ⟨λ (a b : Stream ι α),
 { σ := a.σ × b.σ,
@@ -21,7 +44,48 @@ instance [has_mul α] : has_mul (Stream ι α) := ⟨λ (a b : Stream ι α),
   ready := λ p, Stream.mul.ready a b p,
   skip := λ p hp i r, (a.skip p.1 hp.1 i r, b.skip p.2 hp.2 i r),
   index := λ p hv, max (a.index p.1 hv.1) (b.index p.2 hv.2),
-  value := λ p hr, a.value p.1 hr.r₁ * b.value p.2 hr.r₂ }⟩
+  value := λ p hr, a.value p.1 hr.r₁ * b.value p.2 hr.r₂,
+  wf_rel := prod.rprod_eq a.wf_rel b.wf_rel }⟩
+
+section index_lemmas
+variables [has_mul α]
+
+lemma Stream.mul.ready.index' {a : Stream ι α} {b : Stream ι α} {x y} (h : (a * b).ready (x, y)) :
+  a.index' x = b.index' y :=
+by simp [Stream.index'_val h.v₁, Stream.index'_val h.v₂, h.index]
+
+lemma Stream.mul.ready.order_eq {a : Stream ι α} {b : Stream ι α} {x y} (h : (a * b).ready (x, y)) :
+  a.to_order x = b.to_order y :=
+by ext : 1; simp [h.r₁, h.r₂, h.index']
+
+lemma Stream.mul_index' (a b : Stream ι α) (xy : a.σ × b.σ) :
+  (a * b).index' xy = max (a.index' xy.1) (b.index' xy.2) :=
+begin
+  cases xy with x y,
+  rw [Stream.index'],
+  simp only [Stream.has_mul_mul_index, with_top.coe_max],
+  split_ifs with h,
+  { simp [Stream.index'_val h.1, Stream.index'_val h.2], },
+  erw not_and_distrib at h, cases h; simp [h],
+end
+
+/-- This lemma takes a surprising amount of effort to prove -/
+lemma Stream.min_to_order_le (a b : Stream ι α) (q : a.σ × b.σ) (hv : (a * b).valid q) :
+  min (a.to_order q.1) (b.to_order q.2) ≤ (a * b).to_order q :=
+begin
+  rw prod.lex.le_iff'', 
+  simp only [monotone.map_min (@prod.lex.fst_mono (with_top ι) bool _ _)],
+  split, { convert min_le_max, simp [Stream.mul_index'], },
+  intro h,
+  replace h : a.index' q.1 = b.index' q.2 := by simpa [Stream.mul_index'] using h,
+  suffices : a.ready q.1 → b.ready q.2 → (a * b).ready q,
+  { simpa [Stream.to_order, h, prod.lex.mk_min, bool.min_eq_and, bool.le_iff_imp], },
+  intros hr₁ hr₂,
+  refine ⟨hv.1, hv.2, hr₁, hr₂, _⟩,
+  simpa [hv.1, hv.2] using h,
+end
+
+end index_lemmas
 
 variables [non_unital_non_assoc_semiring α]
 
@@ -29,21 +93,27 @@ variables [non_unital_non_assoc_semiring α]
 def LawfulStream.mul (a b : LawfulStream ι α) : Stream ι α := a.to_Stream * b.to_Stream
 
 namespace LawfulStream.mul
-
-
-local notation a ` ≺ `:50 b := Stream.rel _ a b 
+open Stream
 
 variables {a b : LawfulStream ι α}
 
-def rel {a b : LawfulStream ι α} : (a.σ × b.σ) → (a.σ × b.σ) → Prop :=
-prod.rprod a.rel b.rel
+lemma mul_is_skip_valid : skip_valid_wf (a.mul b) :=
+begin
+  split, { refine prod.rprod_eq_wf a.skip_wf.wf b.skip_wf.wf, },
+  intros q hq i r,
+  rcases a.skip_wf.no_backward q.1 hq.1 i r with (h|⟨ha₁, ha₂⟩),
+  { exact or.inl (or.inl ⟨h, b.skip_wf.no_backward' _ _ _ _⟩), },
+  rcases b.skip_wf.no_backward q.2 hq.2 i r with (h|⟨hb₁, hb₂⟩),
+  { exact or.inl (or.inr ⟨h, a.skip_wf.no_backward' _ _ _ _⟩), },
+  right, split, swap,
+  { dsimp, simp [ha₂, hb₂], },
+  exact lt_of_lt_of_le (lt_min ha₁ hb₁) (Stream.min_to_order_le _ _ _ hq),
+end
 
-local notation a ` ≺ₘ `:50 b := rel a b 
+-- lemma rel_iff  (q₁ q₂ : a.σ × b.σ) :
+--   (q₁ ≺ₘ q₂) ↔ (q₁.1 ≺ q₂.1) ∧ (q₁.2 ≺ q₂.2) := by rw [rel, prod.rprod_iff]
 
-lemma rel_iff  (q₁ q₂ : a.σ × b.σ) :
-  (q₁ ≺ₘ q₂) ↔ (q₁.1 ≺ q₂.1) ∧ (q₁.2 ≺ q₂.2) := by rw [rel, prod.rprod_iff]
-
-lemma rel_wf : well_founded (@rel _ _ _ _ a b) := prod.rprod_wf a.rel_wf b.rel_wf
+-- lemma rel_wf : well_founded (@rel _ _ _ _ a b) := prod.rprod_wf a.rel_wf b.rel_wf
 
 
 
